BVL-->BVP correctness thm sketched

new-backend/bvl_to_bvpScript.sml
@@ -22,8 +22,8 @@ val bComp_def = tDefine "bComp" `
        (Seq c1 c2, HD v1 :: vs, n2)) /\
   (bComp n env tail [Var v] =
      if tail
-     then (Return (index_of v env), [n], n+1)
-     else (Move n (index_of v env), [n], n+1)) /\
+     then (Return (EL v env), [n], n+1)
+     else (Move n (EL v env), [n], n+1)) /\
   (bComp n env tail [If x1 x2 x3] =
      let (c1,v1,n1) = bComp n env F [x1] in
      let (c2,v2,n2) = bComp n1 env tail [x2] in
@@ -61,5 +61,80 @@ val bComp_def = tDefine "bComp" `
      let ret = (if tail then NONE else SOME n1) in
        (Seq c1 (Call ret dest vs), [n1], n+1))`
  (WF_REL_TAC `measure (bvl_exp1_size o SND o SND o SND)`);
+
+val bCompile_def = Define `
+  bCompile arg_count exp =
+    bComp arg_count (GENLIST I arg_count) T [exp]`;
+
+val res_list_def = Define `
+  (res_list (Result x) = Result [x]) /\
+  (res_list (Exception y) = Exception y) /\
+  (res_list TimeOut = TimeOut) /\
+  (res_list Error = Error)`;
+
+val vars_match_def = Define `
+  vars_match vs t xs =
+    EVERY2 (\v x. get_var v t = SOME x) vs xs`;
+
+val var_corr_def = Define `
+  var_corr env corr t <=>
+    (LENGTH corr = LENGTH env) /\
+    !k. k < LENGTH env ==>
+        (get_var (EL k corr) t = SOME (EL k env))`;
+
+val bComp_correct = prove(
+  ``!xs env s1 res s2 t1 n corr tail.
+      (bEval (xs,env,s1) = (res,s2)) /\ res <> Error /\
+      var_corr env corr t1 /\ (LENGTH xs <> 1 ==> ~tail) ==>
+      ?t2 prog pres vs next_var.
+        (bComp n corr tail xs = (prog,vs,next_var)) /\
+        (pEval (prog,t1) = (pres,t2)) /\
+        (case pres of
+         | SOME r => (res_list r = res) /\ (isResult res ==> tail)
+         | NONE => ~tail /\ case res of
+                            | Result xs => vars_match vs t2 xs
+                            | _ => F)``,
+  ONCE_REWRITE_TAC [EQ_SYM_EQ]
+  \\ recInduct bEval_ind \\ REPEAT STRIP_TAC
+  \\ FULL_SIMP_TAC std_ss [bComp_def,pEval_def,bEval_def]
+  THEN1 (* NIL *)
+    (SRW_TAC [] [vars_match_def])
+  THEN1 (* CONS *)
+   (`?c1 v1 n1. bComp n corr F [x] = (c1,v1,n1)` by METIS_TAC [PAIR]
+    \\ `?c2 vs n2. bComp n1 corr F (y::xs) = (c2,vs,n2)` by METIS_TAC [PAIR]
+    \\ FULL_SIMP_TAC std_ss [LET_DEF,pEval_def]
+    \\ Cases_on `bEval ([x],env,s)`
+    \\ Cases_on `q` \\ FULL_SIMP_TAC (srw_ss()) [] THEN1
+     (FIRST_X_ASSUM (MP_TAC o Q.SPECL [`t1`,`n`,`corr`,`F`])
+      \\ FULL_SIMP_TAC std_ss []
+      \\ ONCE_REWRITE_TAC [EQ_SYM_EQ] \\ REPEAT STRIP_TAC
+      \\ Cases_on `pres` \\ FULL_SIMP_TAC std_ss [isResult_def]
+      \\ Cases_on `bEval (y::xs,env,r)`
+      \\ Cases_on `q` \\ FULL_SIMP_TAC (srw_ss()) [isResult_def]
+      \\ FIRST_X_ASSUM (MP_TAC o Q.SPECL [`t2`,`n1`,`corr`,`F`])
+      \\ `var_corr env corr t2` by cheat (* needs stronger ind hyp *)
+      \\ FULL_SIMP_TAC std_ss []
+      \\ ONCE_REWRITE_TAC [EQ_SYM_EQ] \\ REPEAT STRIP_TAC
+      \\ FULL_SIMP_TAC std_ss []
+      \\ cheat (* easy *))
+    \\ RES_TAC
+    \\ POP_ASSUM (MP_TAC o Q.SPECL [`F`,`n`])
+    \\ ASM_REWRITE_TAC [] \\ SIMP_TAC std_ss []
+    \\ ONCE_REWRITE_TAC [EQ_SYM_EQ] \\ REPEAT STRIP_TAC
+    \\ Cases_on `pres` \\ FULL_SIMP_TAC (srw_ss()) [])
+  THEN1 (* Var *)
+   (Cases_on `tail` \\ FULL_SIMP_TAC std_ss []
+    \\ Cases_on `n < LENGTH env`
+    \\ FULL_SIMP_TAC (srw_ss()) [pEval_def]
+    \\ FULL_SIMP_TAC std_ss [var_corr_def,res_list_def]
+    \\ FULL_SIMP_TAC std_ss [vars_match_def,LIST_REL_def]
+    \\ FULL_SIMP_TAC (srw_ss()) [get_var_def,set_var_def])
+  THEN1 (* If *) cheat (* missing case *)
+  THEN1 (* Let *) cheat (* missing case *)
+  THEN1 (* Raise *) cheat (* missing case *)
+  THEN1 (* Handle *) cheat (* missing case *)
+  THEN1 (* Op *) cheat (* missing case *)
+  THEN1 (* Tick *) cheat (* missing case *)
+  THEN1 (* Call *) cheat (* missing case *));
 
 val _ = export_theory();
